---
title: "[Calculus] 14.4 Tangent Planes and Linear Approximation"
categories: [AI, Calculus]
tags: 
math: true
---


> # Tangent Planes

| ![joint](/assets/img/MATH/calculus/ch14_3.png) |
| :-----------------------------------------------: |
|          _stewart-calculus-8th-edition_           |

Suppose a surface $$S$$ has equation $$z=f(x,y)$$ where $$f$$ has continuous first partial derivatives. Let $$P(x_0,y_0,z_0)$$ be a point on $$S$$. Also, let $$C_1$$ and $$C_2$$ be the curves obtained by **intersecting the vertical planes** $$y=y_0$$ and $$x=x_0$$ with the surface $$S$$ as shown in the figure above. Then, the point $$P$$ lies on both $$C_1$$ and $$C_2$$.

Let $$T_1$$ and $$T_2$$ be the **tangent lines** to the curves $$C_1$$ and $$C_2$$ at $$P$$. Then, the **tangent plane** to the surface $$S$$ at the point $$P$$ is the **plane that contains both tangent lines** $$T_1$$ and $$T_2$$.

It can be shown that the **tangent line** of any other curce $$c$$ that lines on the surface $$S$$ passing through $$P$$ **also lies in the tangent plane**. Hence, the tangent plane to $$S$$ at $$P$$ can be interpreted as the plane consisting of **all possible tangent lines** at $$P$$ to curves that lie on $$S$$ passing through $$P$$. The tangent plane at $$P$$ is the plane that **most closely approximates** the surface $$S$$ near the point $$P$$.

The equation for any plan passing through $$P(x_0, y_0, z_0)$$ is

$$ A(x-x_0)+B(y-y_0)+C(z-z_0) = 0 $$

Divide it by $$C$$,

$$ \frac{A}{C}(x-x_0)+\frac{B}{C}(y-y_0)+(z-z_0) = 0 $$

$$ (z-z_0) = -\frac{A}{C}(x-x_0) - \frac{B}{C}(y-y_0) $$

Let $$a = -A/C$$ and $$b = -B/C$$

$$ (z-z_0) = a(x-x_0) + b(y-y_0) $$

If this represents the tangent plane at $$P$$, then its **intersection with the plane** $$y=y_0$$ must be the tangent line $$T_1$$. Hence, we set $$y=y_0$$ and it gives

$$ (z-z_0) = a(x-x_0)\ \text{ where } y=y_0 $$

This is the **point-slope** equation of a line with slope $$a$$. But we know that the slop of the tangent $$T_1$$ is $$f_x(x_0,y_0)$$. Therefore, $$a = f_x(x_0,y_0)$$.

If we operate the same procedure for $$x=x_0$$, we get

$$ (z-z_0) = b(y-y_0)\ \text{ where } x=x_0 $$

where $$b=f_y(x_0,y_0)$$

Finally we can define the equation of the tangent plane.

## Tangent Plane Equation

> Suppose $$f$$ has continuous partial derivatives. An equation of the tangent plane to the surface $$z=f(x,y)$$ at the point $$P(x_0, y_0, z_0)$$ is

$$ z-z_0 = f_x(x_0,y_0)(x-x_0) + f_y(x_0,y_0)(y-y_0) $$

or

$$ z = f(a,b) + f_x(x_0,y_0)(x-x_0) + f_y(x_0,y_0)(y-y_0) $$

## Example

Find the tangent plane to the elliptic paraboloid $$z=2x^2+y^2$$ at the point $$(1,1,3)$$

Let $$f(x,y) = 2x^2+y^2$$. The tangent plane equation is given by $$z-z_0 = f_x(x_0,y_0)(x-x_0) + f_y(x_0,y_0)(y-y_0)$$.

$$ f_x(x,y) = 4x $$

$$ f_y(x,y) = 2y $$

Hence, at $$(1,1,3)$$,

$$ f_x(1,1) = 4 $$

$$ f_y(1,1) = 2 $$

$$ z-3 = 4(x-1) + 2(y-1) $$

$$ \therefore z = 4x+2y-3 $$

> # Linear Approximations

In the above example, we found the tangent plane to the graph of the function $$f(x,y) = 2x^2 + y^2$$. This tangent plane is a good **approximation** to $$f(x,y)$$ when $$(x,y)$$ is **near** $$(1,1)$$. The function $$L$$ is called the **linearization** of $$f$$ at $$(1,1)$$ and the approximation

$$ f(x,y) \approx 4x + 2y - 3 $$

is called the **linear approximation** or **tangent plane approximation** of $$f$$ at $$(1,1)$$.

In general, the tangent plane to $$f$$ (two variables) at $$(a, b, f(a,b))$$ is

$$ z = f(a,b) + f_x(a,b)(x-a) + f_y(a,b)(y-b) $$

Then, we can define **linearization** and **linear approximation**

## Linearization

$$ L(x,y) = f(a,b) + f_x(a,b)(x-a) + f_y(a,b)(y-b) $$

is called the **linearization** of $$f$$ at $$(a,b)$$

## Linear approximation

$$ f(x,y) \approx f(a,b) + f_x(a,b)(x-a) + f_y(a,b)(y-b) $$

is called the **linear approximation** or the **tangent plane approximation** of $$f$$ at $$(a,b)$$.

> # Differentiable

We previously defined tangent plane where $$f$$ has **continuous first partial derivatives**. But if $$f_x$$ and $$f_y$$ are **not continuous**?, we might get a bad approximation. To rule out such behavior, we formulate the idea of **differentiable function** of two variables.

Consider a function of two variables $$z = f(x,y)$$ and suppose $$x$$ changes from $$a$$ to $$a + \Delta x$$ and $$y$$ changes from $$b$$ to $$b + \Delta y$$. THen, the corresponding **increment** of $$z$$ is

$$ \Delta z = f(a + \Delta x, b + \Delta y) - f(a,b) $$

From this, formulate the definition:

## Definition

If $$z=f(x,y)$$, then $$f$$ is **differentiable** at $$(a,b)$$ if $$\Delta z$$ can be expressed in the form

$$ \Delta z = f_x(a,b)\Delta x + f_y(a,b) \Delta + \epsilon_1 \Delta x + \epsilon_2 \Delta y $$

where $$\epsilon_1, \epsilon_2 \rightarrow 0$$ as $$(\Delta x, \Delta y) \rightarrow (0,0)$$

---

A differentiable function is one for which the **linear approximation is a good approximation**.

## Alternative Definition

It's sometimes hard to use the above definition to check differentiablity. The following theorem provides a simpler but sufficient condition for differentiability

> If the partial derivatives $$f_x$$ and $$f_y$$ exist near $$(a,b)$$ and are continuous at $$(a,b)$$, then $$f$$ is differentiable at $$(a,b)$$.

> # Differentials

| ![joint](/assets/img/MATH/calculus/ch14_4.png) |
| :-----------------------------------------------: |
| _single variable (stewart-calculus-8th-edition)_  |

For a differentiable univariate function $$y=f(x)$$, the **differential** $$dx$$ is an **independent variable**; that is, $$dx$$ can be given any real number. The differential of $$y$$ is then defined as

$$ dy = f'(x)dx $$

**[1]** $$\Delta y$$ - change in height of $$y=f(x)$$

**[2]** $$dy$$ - changed in height of the **tangent line** when $$x$$ changes by an amount $$dx = \Delta x$$

| ![joint](/assets/img/MATH/calculus/ch14_5.png) |
| :-----------------------------------------------: |
|          _stewart-calculus-8th-edition_           |

For a differentiable function with **two variables**, $$z = f(x,y)$$, we define the **differentials** $$dx$$ and $$dy$$ to be **independent variables** (any values). Then, the **differential** $$dz$$, also called the **total differential**, is defined by

$$ dz = f_x(x,y)dx + f_y(x,y)dy $$

$$ = \frac{\partial z}{\partial x}dx + \frac{\partial z}{\partial y}dy $$

---

If we take $$dx = \Delta x = x - a$$ and $$dy = \Delta y = y - b$$ in the above equation, then the differential of $$z$$ is

$$ dz = f_x(a,b)(x-a) + f_y(a,b)(y-b) $$

So, we can rewrite the **linear approximation** using differential:

$$ f(x,y) \approx f(a,b) + dx $$

> # References

[1] Stewart Calculus, 8th edition
