---
title: "[Calculus] 14.5 Chain Rule"
categories: [AI, Calculus]
tags: 
math: true
---

> # The Chain Rule

## Single Variable

The chain rule for a single variable gives the rule for differentiating a **composite function**: If $$y=f(x)$$ and $$x=g(t)$$, where $$f$$ and $$g$$ are differentiable functions: $$y=f(g(t))$$

$$ \frac{dy}{dt} = \frac{dy}{dx} \frac{dx}{dt} $$

or

$$ y = f'(g(t)) \cdot g'(t) $$

> # [Chain Rule] Multi-variable: Case 1

Suppose that $$z = f(x,y)$$ is a differentiable function of $$x$$ and $$y$$, where $$x = g(t)$$ and $$y = h(t)$$ are both differentiable functions of $$t$$. Then, $$z$$ is a differentiable function of $$t$$ and

$$ \frac{dz}{dt} = \frac{\partial f}{\partial x}\frac{dx}{dt} + \frac{\partial f}{\partial y}\frac{dy}{dt} $$

Since we often write $$\partial z / \partial x$$ as $$\partial f / \partial x$$, we can rewrite the chain rule as

$$ \frac{dz}{dt} = \frac{\partial z}{\partial x}\frac{dx}{dt} + \frac{\partial z}{\partial y}\frac{dy}{dt} $$

## Example 1

$$z = x^2y + 3xy^4$$ where $$x=\sin{2t}$$ and $$y=\cos{t}$$. Find $$dz/dt$$ when $$t = 0$$

$$ \frac{\partial z}{\partial x} = 2xy + 3y^4,\ \ \frac{dx}{dt} = 2 \cos{2t} $$

$$ \frac{\partial z}{\partial y} = x^2 + 12xy^3,\ \ \frac{dy}{dt} = -\sin{t} $$

Hence,

$$ \frac{dz}{dt} = (2xy+3y^4)(2\cos{2t}) + (x^2 + 12xy^3)(-\sin{t}) $$

Since $$x=0$$ and $$y=1$$ when $$t=0$$,

$$ \frac{dz}{dt} \bigg\vert\_{t=0} = 6 $$

> # [Chain Rule] Multi-variable: Case 2

Suppose $$z = f(x,y)$$ is a differentiable function of $$x$$ and $$y$$, where $$x = g(s,t)$$ and $$y=h(s,t)$$ are differentiable functions of $$s$$ and $$t$$. Then,

$$ \frac{\partial z}{\partial s} = \frac{\partial z}{\partial x}\frac{\partial x}{\partial s} + \frac{\partial z}{\partial y}\frac{\partial y}{\partial s} $$

$$ \frac{\partial z}{\partial t} = \frac{\partial z}{\partial x}\frac{\partial x}{\partial t} + \frac{\partial z}{\partial y}\frac{\partial y}{\partial t} $$

## Independent, Intermediate, Dependent Variables

For Case 2 of the chain rule,

**[1]** $$s$$ and $$t$$ are **independent** variables

**[2]** $$x$$ and $$y$$ are **intermediate** variables

**[3]** $$z$$ is the **dependent** variable

## Example 3

If $$z = e^x\sin{y}$$ where $$x = st^2$$ and $$y=s^2t$$, find $$\partial z/ \partial s$$ and $$\partial z / \partial t$$.

$$ \frac{\partial z}{\partial s} = \frac{\partial z}{\partial x}\frac{\partial x}{\partial s} + \frac{\partial z}{\partial y}\frac{\partial y}{\partial s} = (e^x \sin{y})(t^2) + (e^x \cos{y})(2st) $$

$$ \frac{\partial z}{\partial t} = \frac{\partial z}{\partial x}\frac{\partial x}{\partial t} + \frac{\partial z}{\partial y}\frac{\partial y}{\partial t} = (e^x\sin{y})(2st) + (e^x\cos{y})(s^2) $$

> # [Chain Rule] Multi-variable: General Version

Suppose that $$u$$ is a differentiable function of $$n$$ variables $$x_1,x_2,...,x_n$$ and each $$x_j$$ is a differentiable function of the $$m$$ variables $$t_1,t_2,...,t_m$$. Then $$u$$ is a function of $$t_1, t_2,...,t_m$$ and

$$ \frac{\partial u}{\partial t_i} = \frac{\partial u}{\partial x_i}\frac{\partial x_i}{\partial t_i} + \frac{\partial u}{\partial x_2}\frac{\partial x_2}{\partial t_i}+ \cdots + \frac{\partial u}{\partial x_n}\frac{\partial x_n}{\partial t_i} $$

for each $$i=1,2,...,m$$

> # Tree Diagram

It's often useful to draw tree diagram to visualize the chain rule. Let's take **Case 2**.

$$ \frac{\partial z}{\partial s} = \frac{\partial z}{\partial x}\frac{\partial x}{\partial s} + \frac{\partial z}{\partial y}\frac{\partial y}{\partial s} $$

$$ \frac{\partial z}{\partial t} = \frac{\partial z}{\partial x}\frac{\partial x}{\partial t} + \frac{\partial z}{\partial y}\frac{\partial y}{\partial t} $$

Then, the tree diagram can be drawn as follow,

| ![sdf](..//assets/img/MATH/calculus/ch14_6.png) |
| :---------------------------------------------: |
|          Stewart Calculus, 8th edition          |

## Example 5

If

$$ u = x^4y + y^2z^3 $$

$$ x=rse^t $$

$$ y=rs^2e^{-t} $$

$$ z=r^2s \sin{t} $$

then the tree diagram is

| ![sdf](..//assets/img/MATH/calculus/ch14_7.png) |
| :---------------------------------------------: |
|          Stewart Calculus, 8th edition          |

If we want to find, for example, $$\frac{\partial u}{\partial s}$$, then **add all the "routes"** from $$u$$ to $$s$$.

$$ \frac{\partial u}{\partial s} = \frac{\partial u}{\partial x}\frac{\partial x}{\partial s} + \frac{\partial u}{\partial y}\frac{\partial y}{\partial s} + \frac{\partial u}{\partial z}\frac{\partial z}{\partial s} $$

> # Implicit Differentiation: Case 1

The Chain Rule can be used for implicit differentiation.

Suppose $$F(x,y)=0$$ defines $$y$$ **implicitly** as a differentiable function of $$x$$, that is, $$y=f(x)$$, where $$F(x, f(x))= 0$$ for all $$x$$ in the domain of $$f$$. If $$F$$ is differentiable, we can apply **Case 1** Chain rule to **differentiate both sides of** $$F(x,y) = 0$$ **w.r.t** $$x$$.

$$ \frac{\partial F}{\partial x}\frac{\partial x}{\partial x} + \frac{\partial F}{\partial y}\frac{\partial y}{\partial x} = 0 $$

If $$\partial F / \partial y \neq 0$$, then we can solve for $$dy/dx$$:

$$ \frac{dy}{dx} = -\frac{\frac{\partial F}{\partial x}}{\frac{\partial F}{\partial y}} = -\frac{F_x}{F_y} $$

To derive this equation, we assumed that $$F(x,y)=0$$ defines $$y$$ **implicitly as a function of** $$x$$.

## Example 8

Q) Find $$y'$$ if $$x^3 + y^3 = 6xy$$

---

We can wewrite it as

$$ F(x,y) = x^3 + y^3 - 6xy = 0 $$

Using the equation above,

$$ \frac{dy}{dx} = -\frac{F_x}{F_y} = -\frac{3x^2-6y}{3y^2-6x} = -\frac{x^2 - 2y}{y^2 - 2x} $$

> # Implicit Differentiation: Case 2

Now suppose that $$z$$ is given implicitly as a function of $$z=f(x,y)$$ by an equation of $$F(x,y,z) = 0$$. This means that $$F(x,y,f(x,y))=0$$ for all $$(x,y)$$ in the domain of $$f$$. If $$F$$ and $$f$$ are differentiable, then we can differentiate $$F(x,y,z)$$ **w.r.t** $$x$$ as follows:

$$ \frac{\partial F}{\partial x}\frac{\partial x}{\partial x} + \frac{\partial F}{\partial y}\frac{\partial y}{\partial x} + \frac{\partial F}{\partial z}\frac{\partial z}{\partial x} = 0 $$

But

$$ \frac{\partial}{\partial x} (x) = 1,\ \ \frac{\partial}{\partial x}(y) = 0 $$

Hence, it becomes

$$ \frac{\partial F}{\partial x} + \frac{\partial F}{\partial z}\frac{\partial z}{\partial x} = 0 $$

If $$\partial F / \partial z \neq 0$$, we solve for $$\partial z / \partial x$$:

$$ \frac{\partial z}{\partial x}=-\frac{\frac{\partial F}{\partial x}}{\frac{\partial F}{\partial z}} = -\frac{F_x}{F_z} $$

$$ \frac{\partial z}{\partial y}=-\frac{\frac{\partial F}{\partial y}}{\frac{\partial F}{\partial z}} = -\frac{F_y}{F_z} $$

## Example 8

Find $$\frac{\partial z}{\partial x}$$ and $$\frac{\partial z}{\partial y}$$ if $$x^3+y^3+z^3+6xyz = 1$$.

Let $$F(x,y,z) = x^3+y^3+z^3+6xyz - 1 = 0$$

Then we can use the equatio:

$$ \frac{\partial z}{\partial x} = -\frac{F_x}{F_z} = -\frac{2x^2+6yz}{3z^2+6xy} = -\frac{x^2 + 2yx}{z^2 + 2xy} $$

$$ \frac{\partial z}{\partial y} = -\frac{F_x}{F_z} = -\frac{2y^2+6xz}{3z^2+6xy} = -\frac{y^2 + 2xz}{z^2 + 2xy} $$

> # References

[1] Stewart Calculus, 8th edition
